small_tutorial.ec
@@ -1,0 +1,183 @@
+require import Int CHoareTactic StdBigop.
+import Bigint IntExtra.
+
+(*********************)
+(* Expression's cost *)
+(*********************)
+
+(* Integer constants are free. *)
+lemma free_int : cost(_:{})[true : 1] = 0 by auto.
+
+(* Variable lookups are free. *)
+lemma free_var : cost(_:{x : int})[true : x] = 0 by auto.
+
+(* Same for global variables. *)
+module A = { var x : int }.
+lemma free_var_g : cost(_:{})[true : A.x] = 0 by auto.
+
+(* And logical variables. *)
+lemma free_var_logical (a : int) : cost(_:{})[true : a] = 0 by auto.
+
+(* Everything else has a cost, that must be given by the user through 
+   schemata. A schema allow to quantify over *expressions*, as in: *)
+schema cost_plus {e e' : int}: 
+  cost[true : e + e'] = cost[true : e] + cost[true : e'] + 1.
+
+schema cost_times {e e' : int}: 
+  cost[true : e * e'] = cost[true : e] + cost[true : e'] + 1.
+
+(* It can be instantiated manually with the [instantiate] tactic. *)
+(* Syntax: 
+   instantiate intro_pat := (schema_name memorytype expr1 : expr2 : ...) *)
+lemma foo_cost : cost(_:{})[true : 1 + 2] = 1.
+proof.
+instantiate -> := (cost_plus {} 1 : 2).
+auto.
+qed.
+
+(* Instantiating manually can be avoided using simplification hints.  *)
+hint simplify cost_plus.
+hint simplify cost_times.
+
+lemma foo_cost2 : cost(_:{})[true : 1 + 2] = 1 by auto.
+
+(* Schemata can have type variables, e.g. for lists. *)
+require import List.
+schema cost_cons ['a] {e : 'a} {l : 'a list} : 
+    cost[true : e :: l] =   
+    cost[true : e] + cost[true : l] + 1.
+
+schema cost_nil ['a] : cost[true : [<:'a>]] = 1.
+
+hint simplify cost_cons.
+hint simplify cost_nil.
+lemma foo_list : cost(_:{})[true: [1;2;3;4]] = 5 by auto.
+
+
+(****************************)
+(* Modules and restrictions *)
+(****************************)
+
+
+module B = { 
+  proc g (x, y) : int = {
+    var r : int;
+    r <- x + y;
+    r <- r * x;
+    return r * r;
+  }
+
+  proc f (x : int) : int = {
+    var a : int;
+    a <- x + 1;
+    a <@ g(a,x);
+  return a;
+  }
+}.
+
+(* Assignements are free, only the variable evaluation has a cost. *)
+lemma foo : choare[B.g : true ==> true] time [3].
+proof.
+  proc; auto => * /=.
+qed.
+
+(* Procedure calls are also free. *)
+lemma foo3 : choare[B.f : true ==> true] time [4].
+proof.
+  proc; call foo; auto.
+qed.
+
+module C = { 
+  proc f (x, y) : int = {
+    var r : int;
+    if (y < x) {
+      r <- 1 + 1;
+      r <- 1 + 1;
+     } else {
+      r <- 2 + 1;
+      r <- 2 + 1;
+    }
+    return r;
+  }
+}.
+
+schema cost_lt {e e' : int}: 
+  cost[true : e < e'] = cost[true : e] + cost[true : e'] + 1.
+hint simplify cost_lt.
+
+(* For if statements, to keep cost expressions simpler, we do not use
+    a max. Instead, we add the cost of both branches. *)
+lemma foo4 : choare[C.f : true ==> true] time [5].
+proof.
+proc; auto.
+qed.
+
+module D = { 
+  var g : int
+
+  proc f (x, y) : int = {
+    while (x < y) {
+      x <- x + 1;
+    }
+    return x;
+  }
+}.
+
+lemma foo5 : forall (a : int) (b : int), 
+0 <= a <= b =>
+choare[D.f : x = a /\ y = b /\ x < y ==> true] time [2 * (b - a) + 1].
+proof.
+move => *.
+proc => /=.
+(* The [while] tactic takes the following parameters:
+   - invariant, 
+   - increasing quantity starting from zero
+   - number of loop iterations
+   - cost of one loop body, given using a lambda. *)
+while (x <= y /\ y = b) (x - a) (b - a) [fun _ => 1] => *.
+
+(* prove that the loop body preserves the invariant, and cost what was stated. *)
+auto => * /=; by smt ().
+
+(* prove that the invariant and loop condition implies that we have not reached 
+  the maximal number of steps.  *)
+by smt ().
+
+(* We prove that the invariant implies the post, and that the cost of all
+  iterations is smaller than the final cost. *)
+skip => * => /=; split; [1: by smt].
+rewrite !big_constz !count_predT !size_range; by smt ().
+qed.
+
+
+
+(**************************************************)
+(* Bonus: expression's cost using a free operator *)
+(**************************************************)
+
+op free ['a] (x : 'a) : 'a.
+
+axiom free_id ['a] (x : 'a) : free(x) = x.
+
+schema free_id ['a] {e : 'a} : cost[true : free(e)] = 0.
+
+schema plus_cost_f {e e' : int}: cost[true : free(e) + free(e')] = 1.
+
+(* The schema below is valid for any operator with a call-by-value semantics. *)
+schema plus_cost_e {e e' : int}: 
+  cost[true : e + e'] = 
+  cost[true : free(e) + free(e')] +
+  cost[true : e] + cost[true : e'].
+
+schema free_beta ['a, 'b] {f : 'a -> 'b} {k : 'a} :
+  cost[true : (fun x => f x) k] = 
+  cost[true : f (free k)] + cost[true : k] + 1.
+
+lemma foo_p_f : cost(_:{})[true : 1 + 2] = 1.
+proof.
+instantiate -> := (plus_cost_e {} 1 : 2).
+instantiate -> := (plus_cost_f {} 1 : 2) => //.
+qed.
+
+(* Remark: we cannot use hints there, because plus_cost_e is not terminating. *)
+
